\documentclass[11pt, letterpaper]{article}
\usepackage{fullpage}
\usepackage{amsmath,amsthm,amsfonts,amssymb,amscd}
\usepackage{lastpage}
\usepackage{enumerate}
\usepackage{fancyhdr}
\usepackage{mathrsfs}
\usepackage{enumitem} % \setlist
% for \imageans: float for [H] so the figure floats
\usepackage{graphicx}
\usepackage{adjustbox}
\usepackage{float} 

\setlength{\parindent}{0.25in}
\setlength{\parskip}{0.05in}
% indent paragraphs in list
\setlist{  
  listparindent=\parindent,
  parsep=0pt,
}

% Include graphics in answer
\newcommand{\imageans}[1]
{%
    \begin{figure}[H]
        \centering
        \includegraphics[width=0.4\linewidth]{#1}
    \end{figure}
}

% comments inside align environnment
\newcommand{\comment}[1]{%
  \text{\phantom{(#1)}} \tag{#1}
}
\newtheorem{theorem}{Theorem}
\newtheorem{lemma}{Lemma}
% Cases for Proof environment
\newlist{pcases}{enumerate}{1}
\setlist[pcases]{
  label=\underline{Case~\arabic*}:\protect\thiscase.~,
  ref=\arabic*,
  align=left,
  labelsep=0pt,
  leftmargin=0pt,
  labelwidth=0pt,
  parsep=0pt
}
\newcommand{\case}[1][]{%
  \if\relax\detokenize{#1}\relax
    \def\thiscase{}%
  \else
    \def\thiscase{~#1}%
  \fi
  \item
}

% Edit these as appropriate
\newcommand\course{Math 3124}
\newcommand\hwtitle{HW 4}                  
\newcommand\name{David Tran}
\newcommand\studentid{251169871}

\fancypagestyle{firststyle}
{
    \headheight 35pt
    \lhead{\name}
    \lhead{\name\\\studentid}
    \chead{\textbf{\LARGE \hwtitle}}
    \rhead{\course \\ \today}
    \lfoot{}
    \cfoot{}
    \rfoot{\small\thepage}
    \headsep 1.5em
}

\DeclareUnicodeCharacter{2212}{-}
\begin{document}

\thispagestyle{firststyle}

\setlist[enumerate]{leftmargin=*} % remove enuemrate indentation

\begin{enumerate}
  \item We have $\dot w(t) = \cos t - i \sin t$, so \begin{align*}
    \int_0^{2\pi} \frac{1}{w(t)} \dot w(t) dt 
    &= \int_0^{2\pi} \frac{\cos t - i \sin t}{\sin t + i \cos t} dt \\
    &= \int_0^{2\pi} \frac{(\cos t - i \sin t)(\sin t - i \cos t)}{\sin^2 t + \cos^2 t} dt \\
    &=\int_0^{2\pi} \frac{-i (\sin^2 t + \cos^2 t)}{\sin^2 t + \cos^2 t} dt \\
    &= \int_0^{2\pi} -i dt \\
    &= -2\pi i
  \end{align*}

  This is the negation of the integral parameterized by the previous curve, since $w(t)$ traces out the unit circle in the opposite direction of $z(t)$.

  \item \begin{proof}
    Since $\int_C f(z) dz = re^{i\theta}$ for some $r, \theta \in \mathbb R$, $r = \int_C e^{-i\theta} f(z) dz$. Also, $\vert re^{i \theta} \vert = r = \vert \int_C f(z) dz \vert$, so, using a reparameterization of $z = e^{it}$ for $0 \leq t \leq 2\pi$,
    
    \begin{align*}
      \left\vert \int_C f(z) dz \right\vert 
      &= \int_C e^{-i\theta} f(z) dz \\
      &= \int_0^{2\pi} e^{-i \theta} f(e^{it}) ie^{it} dt \\
      &= \int_0^{2\pi} ie^{i(t - \theta)} f(e^{it}) dt \\
      &= \int_0^{2\pi} (i\cos (t - \theta) + \sin(\theta - t)) f(e^{it}) dt \\
      &\leq \operatorname{Re}\left( \int_0^{2\pi} (i\cos (t - \theta) + \sin(\theta - t)) f(e^{it}) dt \right) \\
      &= \int_0^{2\pi} \sin(\theta - t) f(e^{it}) dt \\
      &\leq \left\vert \int_0^{2\pi} \sin (\theta - t) f(e^{it}) dt \right\vert \\
      &\leq \int_0^{2\pi} \vert \sin(\theta - t) f(e^{it}) \vert dt \\
      &\leq \int_0^{2\pi} \vert \sin(\theta - t) \vert dt\\
      &= 4 
    \end{align*}
    where we use the fact that $\vert f(e^{it}) \vert \leq 1$ in the last inequality.
  \end{proof}

  \newpage

  \item \begin{enumerate}
    \item \begin{proof}
      Let $f(z) = \frac{z^{k + 1}}{k + 1}$. Then $f$ is a function analytic throughout $C$, and $z^k = f'(z)$. So by the Closed Curve Theorem and its corollary, $\int_C z^k dz = 0$.
    \end{proof}

    \item \begin{proof}
      Let $z(\theta) = Re^{i\theta}$. Then $\dot z(\theta) = iRe^{i\theta}$, so
      \begin{align*}
        \int_C z^k dz
        &= \int_0^{2\pi} i(Re^{i \theta})^{k + 1} d\theta \\
        &= \left. \frac{(Re^{i\theta})^{k + 1}}{k + 1} \right\vert_{\theta = 0}^{2\pi} \\
        &= \frac{R^{k + 1}}{k + 1} - \frac{R^{k + 1}}{k + 1} \\
        &= 0
      \end{align*}
    \end{proof}
  \end{enumerate}

  \item \begin{proof}
    Let $a, b \in D$. Define $C: z(t) = (1 - t)a + bt, 0 \leq t \leq 1$. Note then that the start and endpoints of $C$ are $a, b$, respectively. Then by Proposition 4.12, since $f$ is analytic in a convex region, \begin{align*}
      \vert f(b) - f(a) \vert
      &= \left\vert \int_C f'(z) dz \right\vert \\
      &= \left\vert \int_0^1 f'(z(t)) \dot z(t) dt \right\vert \\
      &= \int_0^1 \left\vert f'((1 - t)a + bt) (b - a) \right\vert dt \\
      &\leq \int_0^1 \vert b - a \vert dt \\
      &= \vert b - a \vert
    \end{align*}
    where we use the fact that $\vert f' \vert \leq 1$ in the inequality.
  \end{proof}
\end{enumerate}

\end{document}
