\documentclass[11pt, letterpaper]{article}
\usepackage{fullpage}
\usepackage{amsmath,amsthm,amsfonts,amssymb,amscd}
\usepackage{lastpage}
\usepackage{enumerate}
\usepackage{fancyhdr}
\usepackage{mathrsfs}
\usepackage{enumitem} % \setlist
% for \imageans: float for [H] so the figure floats
\usepackage{graphicx}
\usepackage{adjustbox}
\usepackage{float} 

\setlength{\parindent}{0.25in}
\setlength{\parskip}{0.05in}
% indent paragraphs in list
\setlist{  
  listparindent=\parindent,
  parsep=0pt,
}

% Include graphics in answer
\newcommand{\imageans}[1]
{%
    \begin{figure}[H]
        \centering
        \includegraphics[width=0.4\linewidth]{#1}
    \end{figure}
}

% comments inside align environnment
\newcommand{\comment}[1]{%
  \text{\phantom{(#1)}} \tag{#1}
}
\newtheorem{theorem}{Theorem}
\newtheorem{lemma}{Lemma}
% Cases for Proof environment
\newlist{pcases}{enumerate}{1}
\setlist[pcases]{
  label=\underline{Case~\arabic*}:\protect\thiscase.~,
  ref=\arabic*,
  align=left,
  labelsep=0pt,
  leftmargin=0pt,
  labelwidth=0pt,
  parsep=0pt
}
\newcommand{\case}[1][]{%
  \if\relax\detokenize{#1}\relax
    \def\thiscase{}%
  \else
    \def\thiscase{~#1}%
  \fi
  \item
}

% Edit these as appropriate
\newcommand\course{Math 3122}
\newcommand\hwtitle{HW 1}                  
\newcommand\name{David Tran}
\newcommand\studentid{251169871}

\fancypagestyle{firststyle}
{
    \headheight 35pt
    \lhead{\name}
    \lhead{\name\\\studentid}
    \chead{\textbf{\LARGE \hwtitle}}
    \rhead{\course \\ \today}
    \lfoot{}
    \cfoot{}
    \rfoot{\small\thepage}
    \headsep 1.5em
}

\DeclareUnicodeCharacter{2212}{-}
\begin{document}

\thispagestyle{firststyle}

\setlist[enumerate]{leftmargin=*} % remove enuemrate indentation

\begin{enumerate}
  \item \begin{proof}
    Suppose for the sake of contradiction that such a function $f$ existed. Then $f$ is differentiable so it is continuous. By the MVT, for some $0 < c < x$, $\frac{f(x) - f(0)}{x - 0} = f'(c) = 1$ when $x > 0$. So, $\lim_{x \to 0^+} \frac{f(x) - f(0)}{x} = 1 \neq 0$. Thus, $\lim_{x \to 0}\frac{f(x) - f(0)}{x - 0} \neq 0$, so $f'(0) \neq 0$, contradicting the supposition.
  \end{proof}

  \item \begin{proof}
    Let $F(x) = \int_a^x f(x) dx$. By the Fundamental Theorem of Calculus 2, $F'(x) = f(x)$ and $F$ is continuous. By the MVT, $\frac{F(b) - F(a)}{b - a} = F'(c) = f(c)$ for some $c \in (a, b)$. That is, $F(b) - F(a) = F(b) = \int_a^b f(x) dx = f(c)(b - a)$.
  \end{proof}
\end{enumerate}

\end{document}
